src/Pipit.Exp.Checked.Base.fst
@@ -7,19 +7,13 @@ open Pipit.Prim.Table
 open Pipit.Exp.Base
 open Pipit.Exp.Bigstep
 open Pipit.Exp.Binding
-open Pipit.Exp.Causality
 
 module C  = Pipit.Context.Base
-module CR = Pipit.Context.Row
-module CP = Pipit.Context.Properties
-
 module PM = Pipit.Prop.Metadata
-
-open FStar.Squash
 
 [@@no_auto_projectors]
 noeq
-type check (mode: PM.check_mode) (#t: table) (#c: context t): (#a: t.ty) -> list (row c) -> exp t c a -> Type =
+type check (mode: PM.check_mode) (#t: table u#i u#j) (#c: context t): (#a: t.ty) -> list (row c) -> exp t c a -> Type =
  | CkBase:
           #valty: t.ty ->
           streams: list (row c)    ->
@@ -66,9 +60,9 @@ type check (mode: PM.check_mode) (#t: table) (#c: context t): (#a: t.ty) -> list
           rely: exp t c            t.propty   ->
           guar: exp t (valty :: c) t.propty   ->
           impl: exp t c            valty      ->
-          (PM.prop_status_contains mode status -> bigstep_always streams rely) ->
-          (PM.prop_status_contains mode PM.PSValid ->
-            bigstep_always streams rely ->
+          squash (PM.prop_status_contains mode status ==> bigstep_always streams rely) ->
+          squash (PM.prop_status_contains mode PM.PSValid ==>
+            bigstep_always streams rely ==>
             bigstep_always streams (subst1 guar impl)) ->
           check mode streams rely                  ->
 
@@ -78,7 +72,7 @@ type check (mode: PM.check_mode) (#t: table) (#c: context t): (#a: t.ty) -> list
           // a function impliciation here (`bigstep_always -> check & check`)
           // makes induction difficult.
           // note that bigstep_always is decidable.
-          either (bigstep_always streams rely -> False)
+          either (~ (bigstep_always streams rely))
             (check mode streams impl &
             check mode streams (subst1 guar impl)) ->
 
@@ -89,7 +83,7 @@ type check (mode: PM.check_mode) (#t: table) (#c: context t): (#a: t.ty) -> list
           status:  PM.prop_status                    ->
           eprop:   exp t c             t.propty   ->
           check mode streams                eprop      ->
-          (PM.prop_status_contains mode status ->
+          squash (PM.prop_status_contains mode status ==>
             bigstep_always streams eprop) ->
           check mode streams (XCheck status eprop)
 
@@ -110,13 +104,13 @@ and check_apps (mode: PM.check_mode) (#t: table) (#c: context t): (#a: funty t.t
           check_apps mode streams (XApp f e)
 
 
-let check_all (#t: table) (#c: context t) (#a: t.ty) (mode: PM.check_mode) (e: exp t c a) =
+let check_all (#t: table u#i u#j) (#c: context t) (#a: t.ty) (mode: PM.check_mode) (e: exp t c a) =
   forall (streams: list (row c)).
-    check mode streams e
+    squash (check mode streams e)
 
-let check_apps_all (#t: table) (#c: context t) (#a: funty t.ty) (mode: PM.check_mode) (e: exp_apps t c a) =
+let check_all_apps (#t: table u#i u#j) (#c: context t) (#a: funty t.ty) (mode: PM.check_mode) (e: exp_apps t c a) =
   forall (streams: list (row c)).
-    check_apps mode streams e
+    squash (check_apps mode streams e)
 
 let contract_valid (#t: table) (#c: context t) (#a: t.ty)
   (rely: exp t c t.propty) (guar: exp t (a::c) t.propty) (impl: exp t c a) =
@@ -148,155 +142,3 @@ and bless_apps (#t: table) (#c: context t) (#a: funty t.ty) (e: exp_apps t c a):
   match e with
   | XPrim p -> XPrim p
   | XApp f e -> XApp (bless_apps f) (bless e)
-
-
-let rec lemma_bless_distributes_lift (#t: table) (#c: context t) (#t1: t.ty)
-  (e1: exp t c t1)
-  (ix: C.index_insert c)
-  (t2: t.ty):
-    Lemma
-      (ensures bless (lift1' e1 ix t2) == lift1' (bless e1) ix t2)
-      (decreases e1) =
-  match e1 with
-  | XBase _ -> ()
-  | XApps ea -> lemma_bless_distributes_lift_apps ea ix t2
-  | XFby v e1' -> lemma_bless_distributes_lift e1' ix t2
-  | XMu e1' ->
-    lemma_bless_distributes_lift e1' (ix + 1) t2
-  | XLet b e1' e2' ->
-    lemma_bless_distributes_lift e1'  ix      t2;
-    lemma_bless_distributes_lift e2' (ix + 1) t2
-  | XCheck s e1' ->
-    lemma_bless_distributes_lift e1' ix t2
-  | XContract s r g i ->
-    lemma_bless_distributes_lift r  ix      t2;
-    lemma_bless_distributes_lift g (ix + 1) t2;
-    lemma_bless_distributes_lift i  ix      t2
-
-and lemma_bless_distributes_lift_apps (#t: table) (#c: context t) (#t1: funty t.ty)
-  (e1: exp_apps t c t1)
-  (ix: C.index_insert c)
-  (t2: t.ty):
-    Lemma
-      (ensures bless_apps (lift1_apps' e1 ix t2) == lift1_apps' (bless_apps e1) ix t2)
-      (decreases e1) =
-  match e1 with
-  | XPrim p -> ()
-  | XApp f e ->
-    lemma_bless_distributes_lift_apps f ix t2;
-    lemma_bless_distributes_lift e ix t2
-
-
-
-
-let rec lemma_bless_distributes_subst (#t: table) (#c: context t) (#t1: t.ty)
-  (e1: exp t c t1)
-  (ix: C.index_lookup c)
-  (e2: exp t (C.drop1 c ix) (C.get_index c ix)):
-    Lemma
-      (ensures bless (subst1' e1 ix e2) == subst1' (bless e1) ix (bless e2))
-      (decreases e1) =
-  match e1 with
-  | XBase _ -> ()
-  | XApps ea -> lemma_bless_distributes_subst_apps ea ix e2
-  | XFby v e1' -> lemma_bless_distributes_subst e1' ix e2
-  | XMu e1' ->
-    lemma_bless_distributes_lift  e2 0 t1;
-    lemma_bless_distributes_subst e1' (ix + 1) (lift1 e2 t1)
-  | XLet b e1' e2' ->
-    lemma_bless_distributes_lift  e2 0 b;
-    lemma_bless_distributes_subst e1'  ix      e2;
-    lemma_bless_distributes_subst e2' (ix + 1) (lift1 e2 b)
-  | XCheck s e1' ->
-    lemma_bless_distributes_subst e1' ix e2
-  | XContract s r g i ->
-    lemma_bless_distributes_lift  e2 0 t1;
-    lemma_bless_distributes_subst r  ix      e2;
-    lemma_bless_distributes_subst g (ix + 1) (lift1 e2 t1);
-    lemma_bless_distributes_subst i  ix      e2
-
-and lemma_bless_distributes_subst_apps (#t: table) (#c: context t) (#t1: funty t.ty)
-  (e1: exp_apps t c t1)
-  (ix: C.index_lookup c)
-  (e2: exp t (C.drop1 c ix) (C.get_index c ix)):
-    Lemma
-      (ensures bless_apps (subst1_apps' e1 ix e2) == subst1_apps' (bless_apps e1) ix (bless e2))
-      (decreases e1) =
-  match e1 with
-  | XPrim p -> ()
-  | XApp f e ->
-    lemma_bless_distributes_subst_apps f ix e2;
-    lemma_bless_distributes_subst e ix e2
-
-let rec lemma_bless_of_bigstep (#t: table) (#c: context t) (#a: t.ty) (#streams: list (row c)) (#e: exp t c a) (#v: t.ty_sem a) (hBS: bigstep streams e v):
-  Tot (bigstep streams (bless e) v)
-    (decreases hBS) =
-  admit ()
-
-let rec lemma_bless_of_bigstep_always (#t: table) (#c: context t) (#streams: list (row c)) (#e: exp t c t.propty) (hB: bigstep_always streams e):
-  Tot (bigstep_always streams (bless e))
-    (decreases hB) =
-  admit ()
-
-
-let rec lemma_bigstep_always_of_bless (#t: table) (#c: context t) (#streams: list (row c)) (#e: exp t c t.propty) (hB: bigstep_always streams (bless e)):
-  Tot (bigstep_always streams e)
-    (decreases hB) =
-  admit ()
-
-let rec lemma_check_bless (#t: table) (#c: context t) (#a: t.ty) (#streams: list (row c)) (#e: exp t c a) (hC: check PM.check_mode_all streams e):
-  Tot (check PM.check_mode_valid streams (bless e))
-    (decreases hC) =
-  match hC with
-  | CkBase s b -> CkBase s b
-  | CkApps s ea hCA -> CkApps s (bless_apps ea) (lemma_check_bless_apps hCA)
-  | CkFby1 s v e1 -> CkFby1 s v (bless e1)
-  | CkFbyS l p v e1 hC1 ->
-    CkFbyS l p v _ (lemma_check_bless hC1)
-  | CkMu s e1 hC1 ->
-    lemma_bless_distributes_subst e1 0 (XMu e1);
-    CkMu s (bless e1) (lemma_check_bless hC1)
-  | CkLet s e1 e2 hC1 ->
-    lemma_bless_distributes_subst e2 0 e1;
-    CkLet s (bless e1) (bless e2) (lemma_check_bless hC1)
-  | CkContract s ps r g i hR hG hCr hCig ->
-    lemma_bless_distributes_subst g 0 i;
-
-    let hCig': either (bigstep_always s (bless r) -> False) (check PM.check_mode_valid s (bless i) & check PM.check_mode_valid s (bless (subst1 g i))) =
-      match hCig with
-      | Inl hBN -> Inl (fun hB -> hBN (lemma_bigstep_always_of_bless hB))
-      | Inr (hCi, hCg) -> Inr (lemma_check_bless hCi, lemma_check_bless hCg)
-    in
-    let hR' (pm: PM.prop_status_contains PM.check_mode_valid PM.PSValid) =
-      lemma_bless_of_bigstep_always (hR pm)
-    in
-    let hG' (pm: PM.prop_status_contains PM.check_mode_valid PM.PSValid) (hB: bigstep_always s (bless r)) =
-      lemma_bless_of_bigstep_always (hG pm (lemma_bigstep_always_of_bless hB))
-    in
-    CkContract #PM.check_mode_valid s PM.PSValid (bless r) (bless g) (bless i) hR' hG' (lemma_check_bless hCr) hCig'
-
-  | CkCheck s ps e1 hC1 hB ->
-    let hB' (pm: PM.prop_status_contains PM.check_mode_valid PM.PSValid) =
-      lemma_bless_of_bigstep_always (hB pm)
-    in
-    CkCheck s PM.PSValid (bless e1) (lemma_check_bless hC1) hB'
-
-and lemma_check_bless_apps (#t: table) (#c: context t) (#a: funty t.ty) (#streams: list (row c)) (#ea: exp_apps t c a) (hC: check_apps PM.check_mode_all streams ea):
-  Tot (check_apps PM.check_mode_valid streams (bless_apps ea))
-    (decreases hC)=
-  match hC with
-  | CkPrim s p -> CkPrim s p
-  | CkApp s f e1 hCA hC1 ->
-    CkApp s (bless_apps f) (bless e1)
-      (lemma_check_bless_apps hCA)
-      (lemma_check_bless hC1)
-
-
-let lemma_check_all_bless (#t: table) (#c: context t) (#a: t.ty) (e: exp t c a { check_all PM.check_mode_all e }):
-  Lemma (ensures check_all PM.check_mode_valid (bless e))
-    [SMTPat (check_all PM.check_mode_valid (bless e))] =
-  introduce forall streams. check PM.check_mode_valid streams (bless e)
-  with (
-    eliminate forall streams. check PM.check_mode_all streams e with streams;
-    bind_squash () (fun x -> return_squash (lemma_check_bless x))
-  )
