src/Pipit.System.Exp.Properties.Checked.fst
@@ -1,0 +1,419 @@
+module Pipit.System.Exp.Properties.Checked
+
+open Pipit.Prim.Table
+open Pipit.Exp.Base
+
+module Table = Pipit.Prim.Table
+
+module C  = Pipit.Context.Base
+module CR = Pipit.Context.Row
+
+module SB = Pipit.System.Base
+module SX = Pipit.System.Exp
+module SXP = Pipit.System.Exp.Properties
+
+module X  = Pipit.Exp
+module XB = Pipit.Exp.Bigstep
+module XC = Pipit.Exp.Causality
+module XK = Pipit.Exp.Checked.Base
+
+module PM = Pipit.Prop.Metadata
+
+module List = FStar.List.Tot
+
+module T    = FStar.Tactics
+
+#push-options "--split_queries always"
+
+(*
+   The invariant describes the transition system's state after it has been fed with all of `rows` as inputs.
+*)
+let rec check_invariant
+  (#t: table) (#c: context t) (#a: t.ty)
+  (rows: list (row c))
+  (e: exp t c a { XC.causal e })
+  (mode: PM.check_mode):
+    Tot prop (decreases e) =
+  match e with
+  | XBase _ -> True
+  | XApps e1 -> check_apps_invariant rows e1 mode
+
+  | XFby v1 e2 ->
+    check_invariant rows e2 mode
+
+  | XMu e1 ->
+    check_invariant (CR.zip2_cons (XC.lemma_bigsteps_total_vs rows e) rows) e1 mode
+
+  | XLet b e1 e2 ->
+    check_invariant rows e1 mode /\
+    check_invariant (CR.zip2_cons (XC.lemma_bigsteps_total_vs rows e1) rows) e2 mode
+
+  | XCheck ps e1 ->
+    check_invariant rows e1 mode /\
+    (PM.prop_status_contains mode ps ==> XB.bigstep_always rows e1)
+
+  | XContract ps er eg eb ->
+    let rows' = CR.zip2_cons (XC.lemma_bigsteps_total_vs rows eb) rows in
+    check_invariant rows  er mode /\
+    check_invariant rows' eg mode /\
+    (PM.prop_status_contains mode PM.PSValid ==> XB.bigstep_always rows er ==> XB.bigstep_always rows' eg) /\
+    (PM.prop_status_contains mode ps ==> XB.bigstep_always rows er)
+
+and check_apps_invariant
+  (#t: table) (#c: context t) (#a: funty t.ty)
+  (rows: list (row c))
+  (e: exp_apps t c a { XC.causal_apps e })
+  (mode: PM.check_mode):
+    Tot prop (decreases e) =
+  match e with
+  | XPrim _ -> True
+  | XApp e1 e2 ->
+    check_apps_invariant rows e1 mode /\
+    check_invariant rows e2 mode
+
+let rec check_init
+    (#t: table) (#c: context t) (#a: t.ty)
+    (e: exp t c a { XC.causal e })
+    (mode: PM.check_mode)
+    : Lemma (ensures check_invariant [] e mode)
+      (decreases e) =
+    let tx = SX.system_of_exp e in
+    let rows: list (row c) = [] in
+    match e with
+    | XBase _ -> ()
+
+    | XApps e1 ->
+      check_apps_init e1 (fun r () -> r) mode;
+      ()
+
+    | XFby v1 e2 ->
+      check_init e2 mode
+
+    | XMu e1 ->
+      check_init e1 mode;
+      ()
+
+    | XLet b e1 e2 ->
+      check_init e1 mode;
+      check_init e2 mode;
+      ()
+
+    | XCheck _ e1 ->
+      check_init e1 mode
+
+    | XContract ps er eg eb ->
+      check_init er mode;
+      check_init eg mode;
+      ()
+
+and check_apps_init
+    (#t: table) (#c: context t) (#a: funty t.ty) (#res #inp: Type0)
+    (e: exp_apps t c a { XC.causal_apps e })
+    (f: funty_sem t.ty_sem a -> inp -> res)
+    (mode: PM.check_mode)
+    : Lemma (ensures
+        check_apps_invariant [] e mode)
+      (decreases e) =
+  match e with
+  | XPrim _ -> ()
+  | XApp e1 e2 ->
+    let f' = SX.system_of_exp_apps_distr f in
+    check_apps_init e1 f' mode;
+    check_init e2 mode;
+    ()
+
+
+// let eval_step'
+//     (#t: table) (#c: context t) (#a: t.ty)
+//     (rows: list (row c))
+//     (row1: row c)
+//     (e: exp t c a { XC.causal e })
+//     (s: SB.option_type_sem (SX.state_of_exp e) { SXP.system_of_exp_invariant rows e s })
+//     : Tot (orcl: SB.option_type_sem (SX.oracle_of_exp e) {
+//         let stp = (SX.system_of_exp e).step row1 orcl s in
+//         stp.v == XC.lemma_bigstep_total_v (row1::rows) e /\ SXP.system_of_exp_invariant (row1 :: rows) e stp.s
+//       }) =
+//   let (| v, hBS |) = XC.lemma_bigstep_total (row1 :: rows) e in
+//   SXP.step_invariant_step rows row1 e v hBS s
+
+
+let contract_always_rely
+    (#t: table) (#c: context t) (#a: t.ty)
+    (rows: list (row c))
+    (row1: row c)
+    (ps: PM.contract_status)
+    (er: exp t       c  t.propty { XC.causal er })
+    (eg: exp t (a :: c) t.propty { XC.causal eg })
+    (eb: exp t       c         a { XC.causal eb })
+    : Lemma (requires (
+        check_invariant (row1 :: rows) (XContract ps er eg eb) PM.check_mode_valid /\
+        check_invariant          rows  (XContract ps er eg eb) PM.check_mode_unknown))
+      (ensures (
+        XB.bigstep_always rows er))
+        =
+  // match ps with
+  // | PM.PSUnknown ->
+  //   ()
+  // | PM.PSValid ->
+    ()
+
+
+
+let rec check_step_asm
+    (#t: table) (#c: context t) (#a: t.ty)
+    (rows: list (row c))
+    (row1: row c)
+    (e: exp t c a { XC.causal e })
+    (v: t.ty_sem a)
+    (hBS: XB.bigstep (row1 :: rows) e v)
+    (s: SB.option_type_sem (SX.state_of_exp e) { SXP.system_of_exp_invariant rows e s })
+    : Lemma (requires (
+        check_invariant (row1 :: rows) e PM.check_mode_valid /\
+        check_invariant          rows  e PM.check_mode_unknown))
+      (ensures (
+        let orcl = SXP.step_invariant_step rows row1 e v hBS s in
+        let stp = (SX.system_of_exp e).step row1 orcl s in
+        SB.option_prop_sem stp.chck.assumptions))
+      (decreases e) =
+    let orcl = SXP.step_invariant_step rows row1 e v hBS s in
+    let stp = (SX.system_of_exp e).step row1 orcl s in
+    match e with
+    // | XBase b -> ()
+    // | XApps _ -> admit ()
+    // | XFby v1 e2 ->
+    //   let (| v2, hBS2 |) = XC.lemma_bigstep_total (row1 :: rows) e2 in
+    //   let s: SB.option_type_sem (SB.type_join (Some (t.ty_sem a)) (SX.state_of_exp e2)) = s in
+    //   check_step_asm rows row1 e2 v2 hBS2 (SB.type_join_snd s)
+
+    // | XMu e1 ->
+    //   let (| vs', hBSMus'|) = XC.lemma_bigsteps_total (row1 :: rows) (XMu e1) in
+    //   let XB.BSsS _ _ vs _ _ hBSMus hBSMu = hBSMus' in
+    //   XB.bigstep_deterministic hBS hBSMu;
+    //   let rows' = CR.zip2_cons vs rows in
+    //   let row1' = CR.cons v row1 in
+    //   let hBS1: XB.bigstep (row1' :: rows') e1 v = XC.lemma_bigstep_substitute_elim_XMu (row1 :: rows) e1 (v :: vs) hBSMus' in
+    //   check_step_asm rows' row1' e1 v hBS1 s;
+    //   ()
+
+    // | XLet b e1 e2 ->
+    //   let (| vlefts', hBS1s' |) = XC.lemma_bigsteps_total (row1 :: rows) e1 in
+    //   let XB.BSsS _ _ vlefts _ vleft hBS1s hBS1 = hBS1s' in
+    //   let rows' = CR.zip2_cons vlefts rows in
+    //   let row1' = CR.cons vleft row1 in
+    //   let s: SB.option_type_sem (SB.type_join (SX.state_of_exp e1) (SX.state_of_exp e2)) = s in
+    //   let hBS2 = XC.lemma_bigstep_substitute_elim_XLet (row1 :: rows) e1 vlefts' hBS1s' e2 v hBS in
+    //   assert (check_invariant (row1 :: rows) e1 PM.check_mode_valid);
+    //   assert (check_invariant (row1' :: rows') e2 PM.check_mode_valid);
+    //   check_step_asm rows row1 e1 vleft hBS1 (SB.type_join_fst s);
+    //   check_step_asm rows' row1' e2 v hBS2 (SB.type_join_snd s);
+    //   ()
+
+    // | XCheck ps e1 ->
+    //   // normalize_term_spec (check_invariant (row1 :: rows) (XCheck ps e1) PM.check_mode_valid);
+    //   // norm_spec [delta; zeta; nbe; iota; primops] (check_invariant (row1 :: rows) (XCheck ps e1) PM.check_mode_valid);
+    //   assert (check_invariant (row1 :: rows) e1 PM.check_mode_valid);
+    //   assert (PM.prop_status_contains PM.check_mode_valid ps ==> XB.bigstep_always (row1 :: rows) e1);
+    //   check_step_asm rows row1 e1 s;
+
+    //   let orcl1 = eval_step' rows row1 e1 s in
+    //   let stp1 = (SX.system_of_exp e1).step row1 orcl1 s in
+
+    //   assert (XB.bigstep (row1 :: rows) e1 stp1.v);
+    //   assert (XB.bigstep_always (row1 :: rows) e1 ==> XB.bigstep (row1 :: rows) e1 true);
+    //   if PM.prop_status_contains PM.check_mode_valid ps then
+    //   XB.bigstep_deterministic_squash (row1 :: rows) e1 stp1.v true
+    //   else ();
+    //   ()
+
+
+    | XContract ps er eg eb ->
+      let (| vs', hBSbs' |) = XC.lemma_bigsteps_total (row1 :: rows) eb in
+      let XB.BSsS _ _ vs _ _ hBSbs hBSb = hBSbs' in
+      let XB.BSContract _ _ _ _ _ _ hBSb' = hBS in
+      XB.bigstep_deterministic hBSb hBSb';
+      let rows' = CR.zip2_cons vs rows in
+      let row1' = CR.cons v row1 in
+      let s: SB.option_type_sem (SB.type_join (SX.state_of_exp er) (SX.state_of_exp eg)) = s in
+
+      let (| vr, hBSr |) = XC.lemma_bigstep_total (row1 :: rows)  er in
+      let (| vg, hBSg |) = XC.lemma_bigstep_total (row1' :: rows') eg in
+
+      assert (check_invariant (row1 :: rows) er PM.check_mode_valid);
+      assert (check_invariant (row1' :: rows') eg PM.check_mode_valid);
+      check_step_asm rows row1  er vr hBSr (SB.type_join_fst s);
+      check_step_asm rows' row1' eg vg hBSg (SB.type_join_snd s);
+
+      // assert (XB.bigstep (row1 :: rows) er stp1.v);
+      assert (XB.bigstep_always (row1 :: rows) er ==> XB.bigstep (row1 :: rows) er true);
+      assert (PM.prop_status_contains PM.check_mode_valid PM.PSValid ==> (XB.bigstep_always (row1 :: rows) er ==> XB.bigstep_always (row1' :: rows') eg));
+
+      introduce PM.prop_status_contains PM.check_mode_valid ps ==> b2t vr
+      with pm.
+        XB.bigstep_deterministic_squash (row1 :: rows) er vr true;
+
+      introduce b2t vr ==> b2t vg
+      with hVr. (
+        XB.bigstep_deterministic_squash (row1 :: rows) er vr true;
+        assert (XB.bigstep (row1 :: rows) er true);
+
+        (match ps with
+        | PM.PSValid -> assert (XB.bigstep_always (row1 :: rows) er)
+        | PM.PSUnknown -> assert (XB.bigstep_always rows er));
+        assert (XB.bigstep_always rows er);
+        assert (XB.bigstep_always (row1 :: rows) er)
+        // XB.bigstep_deterministic_squash (row1' :: rows') eg vg true
+      );
+
+
+      // assume (b2t vr ==> b2t vg);
+      // assume (PM.prop_status_contains PM.check_mode_valid ps ==> b2t vr);
+      admit ()
+
+    | _ -> admit ()
+
+//     | XApps e1 ->
+//       let XB.BSApps _ _ _ hBSa = hBS in
+//       let orcl = check_apps_invariant_step rows row1 e1 v hBSa SX.system_of_exp_apps_const () s in
+//       orcl
+
+//     | XFby v1 e2 ->
+//       let (| v2, hBS2 |) = XC.lemma_bigstep_total (row1 :: rows) e2 in
+//       let s: SB.option_type_sem (SB.type_join (Some (t.ty_sem a)) (SX.state_of_exp e2)) = s in
+//       let orcl = check_invariant_step rows row1 e2 v2 hBS2 (SB.type_join_snd s) in
+//       (match hBS with
+//       | XB.BSFby1 _ _ _ ->
+//         orcl
+//       | XB.BSFbyS _ _ _ _ _ hBS' ->
+//       //XXX don't need squash
+//         XB.bigstep_deterministic_squash rows e2 v (SB.type_join_fst s);
+//         orcl)
+
+//     | XMu e1 ->
+//       let (| vs', hBSMus'|) = XC.lemma_bigsteps_total (row1 :: rows) (XMu e1) in
+//       let XB.BSsS _ _ vs _ v' hBSMus hBSMu = hBSMus' in
+//       XB.bigstep_deterministic hBS hBSMu;
+//       assert (vs' == v :: vs);
+//       let rows' = CR.zip2_cons vs rows in
+//       let row1' = CR.cons v row1 in
+//       let s: SB.option_type_sem (SX.state_of_exp e1) = s in
+//       assert (system_of_exp_invariant rows' e1 s);
+
+//       let hBS1: XB.bigstep (row1' :: rows') e1 v = XC.lemma_bigstep_substitute_elim_XMu (row1 :: rows) e1 (v :: vs) hBSMus' in
+
+//       let orcl1 = check_invariant_step rows' row1' e1 v hBS1 s in
+//       let orcl: SB.option_type_sem (SX.oracle_of_exp (XMu e1)) = SB.type_join_tup #(Some (t.ty_sem a)) #(SX.oracle_of_exp e1) v orcl1 in
+
+//       let stp = (SX.system_of_exp (XMu e1)).step row1 orcl s in
+//       assert (system_of_exp_invariant (row1 :: rows) (XMu e1) stp.s);
+//       orcl
+
+//     | XLet b e1 e2 ->
+//       let (| vlefts', hBS1s' |) = XC.lemma_bigsteps_total (row1 :: rows) e1 in
+//       let XB.BSsS _ _ vlefts _ vleft hBS1s hBS1 = hBS1s' in
+//       let rows' = CR.zip2_cons vlefts rows in
+//       let row1' = CR.cons vleft row1 in
+//       let s: SB.option_type_sem (SB.type_join (SX.state_of_exp e1) (SX.state_of_exp e2)) = s in
+//       assert (system_of_exp_invariant rows  e1 (SB.type_join_fst s));
+//       assert (system_of_exp_invariant rows' e2 (SB.type_join_snd s));
+
+//       let hBS2 = XC.lemma_bigstep_substitute_elim_XLet (row1 :: rows) e1 vlefts' hBS1s' e2 v hBS in
+
+//       let orcl1 = check_invariant_step rows  row1  e1 vleft hBS1 (SB.type_join_fst s) in
+//       let orcl2 = check_invariant_step rows' row1' e2 v     hBS2 (SB.type_join_snd s) in
+//       let orcl  = SB.type_join_tup orcl1 orcl2 in
+//       orcl
+
+//     | XCheck _ e1 ->
+//       let XB.BSCheck _ _ _ v1 hBS1 = hBS in
+//       check_invariant_step rows row1 e1 v1 hBS1 s
+
+//     | XContract ps er eg eb ->
+//       let (| vs', hBSbs' |) = XC.lemma_bigsteps_total (row1 :: rows) eb in
+//       let XB.BSsS _ _ vs _ _ hBSbs hBSb = hBSbs' in
+//       let XB.BSContract _ _ _ _ _ _ hBSb' = hBS in
+//       XB.bigstep_deterministic hBSb hBSb';
+//       let rows' = CR.zip2_cons vs rows in
+//       let row1' = CR.cons v row1 in
+//       let s: SB.option_type_sem (SB.type_join (SX.state_of_exp er) (SX.state_of_exp eg)) = s in
+
+//       let (| vr, hBSr |) = XC.lemma_bigstep_total (row1 :: rows)  er in
+//       let (| vg, hBSg |) = XC.lemma_bigstep_total (row1' :: rows') eg in
+
+//       let or = check_invariant_step rows row1  er vr hBSr (SB.type_join_fst s) in
+//       let og = check_invariant_step rows' row1' eg vg hBSg (SB.type_join_snd s) in
+//       let orcl = SB.type_join_tup #(Some (t.ty_sem a)) v (SB.type_join_tup or og) in
+
+//       orcl
+
+// and check_apps_invariant_step
+//     (#t: table) (#c: context t) (#a: funty t.ty) (#res #inp: Type0)
+//     (rows: list (row c))
+//     (row1: row c)
+//     (e: exp_apps t c a { XC.causal_apps e })
+//     (v: funty_sem t.ty_sem a)
+//     (hBS: XB.bigstep_apps (row1 :: rows) e v)
+//     (f: funty_sem t.ty_sem a -> inp -> res)
+//     (inp0: inp)
+//     (s: SB.option_type_sem (SX.state_of_exp_apps e) { system_of_exp_apps_invariant rows e s })
+//     : Tot (orcl: SB.option_type_sem (SX.oracle_of_exp_apps e) {
+//         let stp = (SX.system_of_exp_apps e f).step (inp0, row1) orcl s in
+//         stp.v == f v inp0 /\
+//         system_of_exp_apps_invariant (row1 :: rows) e stp.s
+//       })
+//       (decreases e) =
+//   match e with
+//   | XPrim _ -> ()
+//   | XApp e1 e2 ->
+//     let XB.BSApp _ _ _ v1 v2 hBS1 hBS2 = hBS in
+//     let f' = SX.system_of_exp_apps_distr f in
+//     let s: SB.option_type_sem (SB.type_join (SX.state_of_exp e2) (SX.state_of_exp_apps e1)) = s in
+//     let orcl2 = check_invariant_step      rows row1 e2 v2 hBS2 (SB.type_join_fst s) in
+//     let orcl1 = check_apps_invariant_step rows row1 e1 v1 hBS1 f' (v2, inp0) (SB.type_join_snd s) in
+//     let orcl = SB.type_join_tup orcl2 orcl1 in
+//     orcl
+
+
+// let rec system_invariant_many
+//     (#t: table) (#c: context t) (#a: t.ty)
+//     (inputs: list (row c))
+//     (e: exp t c a { XC.causal e })
+//     : Tot (
+//         state:   SB.option_type_sem (SX.state_of_exp e) { system_of_exp_invariant inputs e state } &
+//         oracles: list (SB.option_type_sem (SX.oracle_of_exp e)) { List.length oracles == List.length inputs } &
+//         results: list (t.ty_sem a) { List.length results == List.length inputs } &
+//         XB.bigsteps inputs e results &
+//         squash (
+//           SB.system_steps (SX.system_of_exp e) inputs oracles == (state, results)
+//         )) =
+//     let t = SX.system_of_exp e in
+//     match inputs with
+//     | [] ->
+//       check_init e;
+//       assert (SB.system_steps (SX.system_of_exp e) inputs [] == (t.init, []));
+//       (| t.init, [], [], XB.BSs0 e, () |)
+//     | i :: inputs' ->
+//       let (| s, oracles, results, hBSs, prf |) = system_invariant_many inputs' e in
+//       let (| r, hBS |) = XC.lemma_bigstep_total (i :: inputs') e in
+//       let o = step_invariant_step inputs' i e r hBS s in
+//       let stp = t.step i o s in
+//       assert (SB.system_steps (SX.system_of_exp e)       inputs'        oracles  == (    s,      results));
+//       assert (SB.system_steps (SX.system_of_exp e) (i :: inputs') (o :: oracles) == (stp.s, r :: results));
+//       assert (SB.system_steps (SX.system_of_exp e)       inputs   (o :: oracles) == (stp.s, r :: results));
+//       let hBSs': XB.bigsteps (i :: inputs') e (r :: results) = XB.BSsS _ e _ _ _ hBSs hBS in
+//       (| stp.s, o :: oracles, r :: results, hBSs', () |)
+
+
+// (* Section 4, Theorem 4, translation-abstraction *)
+// let system_translation_abstraction
+//     (#t: table) (#c: context t) (#a: t.ty)
+//     (inputs: list (row c))
+//     (e: exp t c a { XC.causal e })
+//     (results: list (t.ty_sem a) { List.length results == List.length inputs })
+//     (hBSs: XB.bigsteps inputs e results)
+//     : Tot (oracles: list (SB.option_type_sem (SX.oracle_of_exp e)) {
+//           List.length oracles == List.length inputs /\
+//           snd (SB.system_steps (SX.system_of_exp e) inputs oracles) == results
+//       }) =
+//   let (| s, oracles, results', hBSs', prf |) = system_invariant_many inputs e in
+//   XB.bigsteps_proof_equivalence hBSs hBSs';
+//   oracles
